Working on proof of compiler correctness

843/stack_compiler.v
@@ -7,12 +7,23 @@ Require Import Coq.Lists.List.
 Inductive id : Type :=
 | Id : nat -> id.
 
+Definition state := id -> nat.
+
 Inductive aexp : Type :=
 | ANum : nat -> aexp
 | AId : id -> aexp
 | APlus : aexp -> aexp -> aexp
 | AMinus : aexp -> aexp -> aexp
 | AMult : aexp -> aexp -> aexp.
+
+Fixpoint aeval (st : state) (a : aexp) : nat :=
+  match a with
+  | ANum n => n
+  | AId i => st i       
+  | APlus l r => (aeval st l) + (aeval st r)
+  | AMinus l r => (aeval st l) - (aeval st r)
+  | AMult l r => (aeval st l) * (aeval st r)
+  end.
 
 Theorem eq_id_dec : forall i j : id, {i = j} + {i <> j}.
 intros.
@@ -21,8 +32,6 @@ destruct (eq_nat_dec n n0).
 left. rewrite e. reflexivity.
 right. intros contra. inversion contra. contradiction.
 Defined.
-
-Definition state := id -> nat.
 
 Definition empty_state : state :=
   fun _ => 0.
@@ -45,11 +54,11 @@ Fixpoint s_execute (st : state) (stack : list nat) (prog: list sinstr) : list na
     | SPush n => s_execute st (n :: stack) rest
     | SLoad i => s_execute st ((st i) :: stack) rest
     | SPlus =>
-       (s_execute st (((hd 0 stack) + (hd 0 (tl stack))) :: (tl (tl stack))) rest)
+       (s_execute st (((hd 0 (tl stack)) + (hd 0 stack)) :: (tl (tl stack))) rest)
     | SMinus =>
       (s_execute st (((hd 0 (tl stack)) - (hd 0 stack)) :: (tl (tl stack))) rest)
     | SMult =>
-       (s_execute st (((hd 0 stack) * (hd 0 (tl stack))) ::(tl (tl stack))) rest)
+       (s_execute st (((hd 0 (tl stack)) * (hd 0 stack)) ::(tl (tl stack))) rest)
     end                  
   end.
 
@@ -80,4 +89,19 @@ Example s_compile1 :
   s_compile (AMinus (AId (Id 1)) (AMult (ANum 2) (AId (Id 2))))
   = [SLoad (Id 1), SPush 2, SLoad (Id 2), SMult, SMinus].
 reflexivity.
+Qed.
+
+Lemma execute_compile : forall st e1 e2 e3 , s_execute st [] (e1 ++ e2 ++ e3) = s_execute st ((s_execute st [] e2) ++ (s_execute st [] e1)) e3.
+  intros. induction e1. simpl. induction e2.
+  reflexivity.
+  induction a. simpl.
+  Admitted.
+  
+Theorem s_compile_correct : forall st a, s_execute st [] (s_compile a) = [ (aeval st a) ].
+intros. induction a.
+reflexivity.
+reflexivity.
+simpl. rewrite execute_compile. rewrite IHa1. rewrite IHa2. reflexivity.
+simpl. rewrite execute_compile. rewrite IHa1. rewrite IHa2. reflexivity.
+simpl. rewrite execute_compile. rewrite IHa1. rewrite IHa2. reflexivity.
 Qed.
